---
title: "GEOS 568: Advanced Seismology HW2. Due: 10/24/24"
subtitle: "Name: Joses Omojola"
output:
  pdf_document: default
header-includes:
  - \usepackage{amsmath}
---

1. Solve the wave equation below using the method of separation of variables. Here $\phi$ is a scalar field.
$$
\frac{\partial^2 \phi}{\partial t^2} = c^2 \nabla^2 \phi
$$

__Proof__  
Let $\phi(x,t)$ represent displacement from the $x$ axis at position $x$ and time $t$. $\nabla^2$ is the Laplacian operator for spatial 
coordinates, and can be rewritten as  $\frac{\partial^2 \phi}{\partial t^2}(x,t)$. 
<!-- Laplacian is the divergence of the gradient -->

Boundary conditions  
The displacement at the left and right are held at zero  
\begin{align}
&\phi(0,t) = 0  & \text{for all } t > 0 \\
&\phi(l,t) = 0  & \text{for all } t > 0
\end{align}

Initial conditions  
The postion and speed of the wave at time 0 is represented by functions $f(x)$ and $g(x)$
\begin{align}
&\phi(x,0) = f(x)  & \text{for all } 0 < x < l \\
&\phi(x,0) = g(x)  & \text{for all } 0 < x < l
\end{align}
  
Using the separation of variables method, we start by finding all solutions of the original equation of the form $\phi(x,t) = X(x)T(t)$. Then 
we impose the boundary conditions, and the initial conditions.  
The original equation can be rewritten as 
\begin{align*}
\phi_{tt} = X(x)T''(t) \\
\phi_{xx} = X''(x)T(t) \\
X(x)T''(t) = c^2 X''(x)T(t) \\ 
\text{grouping like terms} \\
\frac{X''(x)}{X(x)} = \frac{1}{c^2}\frac{T''(t)}{T(t)}
\end{align*}
Both sides are independent of each other and equal, indicating that they are equal to a constant which can be represented as $\lambda$.
\begin{gather}
\tag{5}
\begin{aligned}
\frac{X''(x)}{X(x)} & = \lambda  & \frac{1}{c^2}\frac{T''(t)}{T(t)} = \lambda \\
\Longleftrightarrow X''(x) - \lambda X(x) & = 0 & T''(t) - c^2 \lambda T(t) = 0
\end{aligned}
\end{gather}

We can solve the two constant coefficient ordinary differential equations, by trying $X(x)=e^{rx}$ and $T(t)=e^{st}$ for some constants r and s 
to be determined. These solution only hold if  and only if
$$
\begin{array}{lrrr}
&  & \frac{d^2}{dx^2}e^{rx} - \lambda e^{rx} = 0    & \frac{d^2}{dt^2}e^{st} - c^2 \lambda e^{st} = 0 \\
& \Longleftrightarrow & (r^2 - \lambda)e^{rx} = 0     & (s^2 - c^2 \lambda)e^{st} = 0 \\
& \Longleftrightarrow & r^2 - \lambda = 0             & s^2 - c^2 \lambda = 0 \\
& \Longleftrightarrow & r = \pm \sqrt{\lambda}        & s = \pm c\sqrt{\lambda}
\end{array}
$$
If $\lambda \neq 0$, we obtain two independent solutions, namely $e^{\sqrt{\lambda} x}$ and $e^{-\sqrt{\lambda} x}$ for $X(x)$, and two independent 
solutions namely, $e^{c\sqrt{\lambda} t}$ and $e^{-c\sqrt{\lambda} t}$ for $T(t)$. If $\lambda \neq 0$, the general solution to (5) is
\begin{align*}
& X(x) = d_1 e^{\sqrt{\lambda} x} + d_2 e^{-\sqrt{\lambda} x}   & T(t) = d_3 e^{c\sqrt{\lambda} t} + d_4 e^{-c\sqrt{\lambda} t}
\end{align*}
for arbitrary constants $d_1, d_2, d_3, \text{ and } d_4$. If $\lambda \neq 0$, equation (5) can be simplified to 
\begin{align*}
& X''(x) = 0   & T''(t) = 0
\end{align*}
and the general solution is
\begin{align*}
& X(x) = d_1 + d_2 x   & T(t) = d_3 + d_4 x
\end{align*}

We proceed by imposing the bounding conditions in (1) and (2) above. If $X_i(x)T_i(t), \ i=1,2,3,...$ all solve the wave equation, then 
$\Sigma_i a_iX_i(x)T_i(t)$ is also a solution for any choice of the constant $a_i$. This solution satisfies the boundary condition (1) if and 
only if
$$
\sum_i a_i X_i(0)T_i(t) = 0 \ \ \ \  \text{ for all }t > 0
$$
Similarly $\phi(x,t) = \Sigma_i a_iX_i(x)T_i(t)$ satisfies the boundary condition (2) if and only if 
$$
\sum_i a_i X_i(l)T_i(t) = 0 \ \ \ \  \text{ for all }t > 0
$$
By iterating through the solutions of coefficient ordinary differential equations, we can discard all of those that fail to satisfy 
$X(0) = X(l) = 0$. We consider $\lambda \neq 0$. The condition $X(0)=0$ is satisfied if and only if $d_1 + d_2 = 0$. So we require that $d_2 = -d_1$.
The condition $X(l)=0$ is satisfied if and only if
$$
0 = d_1 e^{\sqrt{\lambda} t} + d_2 e^{-\sqrt{\lambda} t} = d_1 \left( e^{\sqrt{\lambda} t} - e^{-\sqrt{\lambda} t} \right)
$$
If $d_1$ were zero, then $X(x)$ would again be identically zero and hence useless. So instead, we discard any $\lambda$ that doesn't obey.
$$
e^{\sqrt{\lambda} l} - e^{-\sqrt{\lambda} l} = 0 \Longleftrightarrow e^{\sqrt{\lambda} l} = e^{-\sqrt{\lambda} l} 
\Longleftrightarrow e^{2 \sqrt{\lambda} l} = 1
$$
In the last step, we multiplied both sides of $e^{\sqrt{\lambda} l}$. One $\lambda$ that obeys $e^{2 \sqrt{\lambda} l} = 1$ is $\lambda = 0$. Since 
we're only considering $\lambda \neq 0$, we can't use it, however, there are infinitely many complex numbers that work. In fact 
$e^{2 \sqrt{\lambda} l} = 1$ if and only if there is an integer $k$ such that 
$$
2 \sqrt{\lambda} l = 2 k \pi l \Longleftrightarrow \sqrt{\lambda} = k \frac{\pi}{l} l \Longleftrightarrow \lambda = -k^2 \frac{\pi^2}{l^2}
$$ 
With $\sqrt{\lambda} = k \frac{\pi}{l} l$ and $d_2 = -d_1$
\begin{align*}
X(x)T(t) &= d_1 \left( e^{l \frac{k \pi}{l} x} - e^{-l \frac{k \pi}{l} x} \right) (d_3 e^{l \frac{ck \pi}{l} t} + d_4 e^{-l \frac{ck \pi}{l} t}) \\
&= 2 l d_1 \sin \left( \frac{k \pi}{l} x \right) \left[ (d_3 + d_4) \cos \left( \frac{ck \pi}{l} t \right) + l(d_3 - d_4) \sin \left( \frac{ck \pi}{l} t \right) \right] \\
&= \sin \left( \frac{k \pi}{l} x \right) \left[ \alpha_k \cos \left( \frac{ck \pi}{l} t \right) + \beta_k \sin \left( \frac{ck \pi}{l} t \right) \right]
\end{align*}
where $\alpha_k = 2l d_1 (d_3 + d_4)$ and $\beta_k = -2 d_1 (d_3 - d_4)$. Note that, to this point, $d_1, d_3, \text{ and } d_4$ are allowed to be 
any complex numbers so that $\alpha_k$ and $\beta_k$ are allowed to be any complex numbers.  

We now know that 
$$
u(x,t) = \sum_{k=1}^{\infty} sin \left(\frac{k\pi}{l}x\right) \left[ \alpha_k cos \left(\frac{ck\pi}{l}t\right) + \beta_k sin \left(\frac{ck\pi}{l}t\right) \right]
$$
obeys the wave equation and the boundary conditions (1) and (2), for any choice of the constants $\alpha_k, \beta_k$. It remains only to see if we can 
choose the $\alpha_k$'s and $\beta_k$'s to satisfy
\begin{align}
& f(x) = u(x,0) = \sum_{k=1}^{\infty} \alpha_k sin \left(\frac{k\pi}{l}x \right) \\
& g(x) = u_t(x,0) = \sum_{k=1}^{\infty} \beta_k \frac{ck\pi}{l} sin \left(\frac{k\pi}{l}x \right)
\end{align}
But any (reasonably smooth) function, $h(x)$, defined on the interval $0 < x < l$, has a unique representation
\begin{equation}
h(x) = \sum_{k=1}^{\infty} b_k sin \frac{k\pi x}{l}
\end{equation}
as a linear combination of $sin \frac{k\pi x}{l}$'s and we also know the formula
$$
b_k = \frac{2}{l} \int_0^l h(x) sin \frac{k\pi x}{l} dx
$$
for the coefficients. We can make (7) match (5) by choosing $h(x) = f(x)$ and $b_k = \alpha_k$. This tells us that 
$\alpha_k = \frac{2}{l} \int_0^l f(x) sin \frac{k\pi x}{l} dx$. Similarly, we can make (7) match (6) by choosing $h(x) = f(x)$ and 
$b_k = \beta_k \frac{ck\pi}{l}$. This tells us that $\frac{ck\pi}{l} \beta_k = \frac{2}{l} \int_0^l g(x) sin \frac{k\pi x}{l} dx$. So we have a solution:
\begin{equation}
\phi(x,t) = \sum_{k=1}^{\infty} sin (\frac{k\pi}{l}x) \left[\alpha_k cos (\frac{ck\pi}{l} t) + \beta_k sin (\frac{ck\pi}{l} t) \right]
\end{equation}
with 
\begin{align*}
& \alpha_k = \frac{2}{l} \int_0^l f(x) sin \frac{k\pi x}{l} dx  & \beta_k = \frac{2}{ck\pi} \int_0^l g(x) sin \frac{k\pi x}{l} dx 
\end{align*}
  
---

\vspace{10em}
  

2. Using AR Box 4.1, prove that \( g(x,t) = \frac{1}{4 \pi c^2 |x|} \delta \left(t - \frac{|x|}{c} \right) \) is the solution to 
\( \ddot{g} = \delta(x)\delta(t) + c^2 \nabla^2 g \). Show your work and include all of the details that are absent from the proof 
in Box 4.1.

__Proof__ 
\begin{enumerate} 
\item[i] In the wave equation \( \ddot{g} = \delta(x)\delta(t) + c^2 \nabla^2 g \), $\ddot{g}$ represents the second time derivative of  $g(x,t)$, and $\nabla^2 g$ represents the Laplacian 
of $g(x,t)$ in space. The term $\delta(x)\delta(t)$ represents a source term localized at $x=0$ and $t=0$, corresponding to a point source.  
\item[ii] Assuming zero initial conditions and a radially symmetric point source at $x=0$. The source is located at the origin and has no preferred direction in space,
hence the solution only depends on the distance from the origin, i.e. $r = |x|$, and not individual coordinates $(x_1,x_2,x_3)$.  
\item[iii] When $\mathbf{g}$ is radially symmetric, the Laplacian $\nabla^2 g$ for a function $g = g(r, t )$ that depends only on the radial coordinate $r$ and time $t$
is given by
$$
\nabla^2 g = \frac{1}{r^2}\frac{\partial}{\partial r} \left(r^2 \frac{\partial g}{\partial r}\right)
$$
\item[iv] The Laplacian can be expanded to:
$$
\nabla^2 g = \frac{1}{r^2} \frac{\partial}{\partial r} \left( r^2 \frac{\partial g}{\partial r} \right) = 
\frac{1}{r^2} \left( 2r \frac{\partial g}{\partial r} + r^2 \frac{\partial^2 g}{\partial r^2} \right) =
\frac{2}{r} \frac{\partial g}{\partial r} + \frac{\partial^2 g}{\partial r^2}
$$

\item[v] The expression for \( \nabla^2 g \) can be substituted into the 3D wave equation:
$$
\ddot{g} = c^2 \left( \frac{2}{r} \frac{\partial g}{\partial r} + \frac{\partial^2 g}{\partial r^2} \right) = 
\frac{2c^2}{r} \frac{\partial g}{\partial r} + c^2 \frac{\partial^2 g}{\partial r^2}
$$

\item[vi] Considering \( h(r, t) = r g(r, t) \), we can express the wave equation in terms of \( h \), and compute the spatial derivatives of \( h \) with respect to \( r \):
$$
g = \frac{h}{r}, \quad \frac{\partial g}{\partial r} = \frac{1}{r} \frac{\partial h}{\partial r} - \frac{h}{r^2}
$$
Substituting these into the expression for \( \nabla^2 g \), the first term becomes:
$$
\frac{2}{r} \frac{\partial g}{\partial r} = \frac{2}{r} \left( \frac{1}{r} \frac{\partial h}{\partial r} - \frac{h}{r^2} \right) = \frac{2}{r^2} \frac{\partial h}{\partial r} - \frac{2h}{r^3}
$$
and the second term:
$$
\frac{\partial^2 g}{\partial r^2} = \frac{\partial}{\partial r} \left( \frac{1}{r} \frac{\partial h}{\partial r} - \frac{h}{r^2} \right)
$$
This expands as:
$$
\frac{\partial^2 g}{\partial r^2} = \frac{1}{r} \frac{\partial^2 h}{\partial r^2} - \frac{2}{r^2} \frac{\partial h}{\partial r} + \frac{2h}{r^3}
$$
Substituting these into the wave equation gives:
$$
\ddot{g} = c^2 \left( \frac{2}{r^2} \frac{\partial h}{\partial r} - \frac{2h}{r^3} + \frac{1}{r} \frac{\partial^2 h}{\partial r^2} - \frac{2}{r^2} \frac{\partial h}{\partial r} + \frac{2h}{r^3} \right)
$$
that can be simplified to:
$$
\ddot{g} = c^2 \frac{1}{r} \frac{\partial^2 h}{\partial r^2}
$$

\item[vii] The wave equation can be expressed in terms of \( h = rg \), since \( g = \frac{h}{r} \):
$$
\ddot{g} = \frac{c^2}{r} \frac{\partial^2 h}{\partial r^2}
$$
Because \( h = r g \), so this equation becomes:
$$
\ddot{g} = \frac{1}{r} \frac{\partial^2 (r g)}{\partial r^2}
$$
The resulting $(rg)''$:
$$
(rg)'' = \frac{r \ddot{g}}{c^2}
$$
satisfies the one-dimensional wave equation.

\item[viii] The general solution to \( r g \) can be represented as 
\[
r g(r, t) = f\left(t - \frac{r}{c}\right) + h\left(t + \frac{r}{c}\right)
\]
where \( f \) represents an outgoing wave and \( h \) represents an incoming wave. Since we are concerned with only the outgoing waves from the source at \( r = 0 \), we set 
\( h(t + \frac{r}{c}) = 0 \), hence 
\[
r g(r, t) = f\left( t - \frac{r}{c} \right)
\]
and $\mathbf{g}$ can be represented as 
\[
g(r, t) = \frac{1}{r} f\left( t - \frac{r}{c} \right)
\]

\item[ix] To show that \( f(\tau) = \frac{\delta(\tau)}{4 \pi c^2} \), where \( \tau = t - \frac{r}{c} \), We must establish that \( 4 \pi c^2 f(\tau) \) has the same properties as 
the Dirac delta function \( \delta(\tau) \) when integrated over time. We introduce the function:
\[
F(r, \epsilon_1, \epsilon_2) \equiv 4 \pi c^2 \int_{\frac{r}{c} - \epsilon_1}^{\frac{r}{c} + \epsilon_2} g(r, t) \, dt
\]
Substitute \( g(r,t) = \frac{1}{r} f\left( t - \frac{r}{c} \right) \) into this expression:
\[
F(r, \epsilon_1, \epsilon_2) = 4 \pi c^2 \int_{\frac{r}{c} - \epsilon_1}^{\frac{r}{c} + \epsilon_2} \frac{1}{r} f\left( t - \frac{r}{c} \right) \, dt
\]
Performing change of variables \( \tau = t - \frac{r}{c} \), \( dt = d\tau \) and the integration limits change to:
\[
F(r, \epsilon_1, \epsilon_2) = \frac{4 \pi c^2}{r} \int_{-\epsilon_1}^{\epsilon_2} f(\tau) \, d\tau
\]

\item[x] We apply the Laplacian \( \nabla^2 \) to \( F(r, \epsilon_1, \epsilon_2) \). Using the definition of \( F \) and the properties of \( g(r, t) \), we need to differentiate both 
the limits of integration and the integrand \( g(r, t) \) with respect to \( r \). The expression for \( \nabla^2 F \) becomes:
\[
\nabla^2 F = 4 \pi c \left[ 2g'(r,t) + \frac{2}{r} g(r, t) + \frac{\dot{g}(r,t)}{c} \right]_{t = \frac{r}{c} + \epsilon_2}^{t = \frac{r}{c} - \epsilon_1}
+ 4 \pi c^2 \int_{\frac{r}{c} - \epsilon_1}^{\frac{r}{c} + \epsilon_2} \nabla^2 g(r, t) \, dt
\]

\item[xi] Substitute the wave equation $\ddot{g} = c^2 \nabla^2 g + \delta(x)\delta(t)$ to replace $\nabla^2 g$ in the integral to get
\begin{align*}
\nabla^2 F &= 4 \pi c \left[ 2g'(r,t) + \frac{2}{r} g(r, t) + \frac{\dot{g}(r,t)}{c} \right]_{\frac{r}{c} + \epsilon_2}^{\frac{r}{c} - \epsilon_1}
+ 4 \pi c^2 \int_{\frac{r}{c} - \epsilon_1}^{\frac{r}{c} + \epsilon_2} \left( \frac{\ddot{g}}{c^2} - \delta(x)\delta(t) \right) \, dt \\
&= 4 \pi c \left[ 2g'(r,t) + \frac{2}{r} g(r, t) + \frac{\dot{g}(r,t)}{c} \right]_{\frac{r}{c} + \epsilon_2}^{\frac{r}{c} - \epsilon_1}
+  4 \pi c^2 \int_{\frac{r}{c} - \epsilon_1}^{\frac{r}{c} + \epsilon_2} \frac{\ddot{g}}{c^2} \, dt 
-  4 \pi c^2 \int_{\frac{r}{c} - \epsilon_1}^{\frac{r}{c} + \epsilon_2} \delta(x)\delta(t) \, dt 
\end{align*}
For $r \neq 0$, the solution $g(r,t)$ satisfies the homogenous equation t

Considering the initial conditions at zero, the contribution of the green's function in the second term integrates to zero. In the third term, since $\delta(x)$ is a function of space, integrating it 
with respect to time will not affect it, and we can pull it out. 
\[
\nabla^2 F = 4 \pi c \left[ 2g'(r,t) + \frac{2}{r} g(r,t) + \frac{\dot{g}(r,t)}{c} \right]_{\frac{r}{c} + \epsilon_2}^{\frac{r}{c} - \epsilon_1}
- 4 \pi \delta(x) \int_{\frac{r}{c} - \epsilon_1}^{\frac{r}{c} + \epsilon_2} \delta(t) \, dt
\]

\item[xii] Using the fact that \( rg = f\left(t - \frac{r}{c}\right) \), which implies that:
\[
g'(r,t) = -\frac{g(r,t)}{r} - \frac{\dot{g}(r,t)}{c}
\]
Substituting this into the equation for \( \nabla^2 F \), we find that all the terms involving \( g(r,t) \), \( g'(r,t) \), and \( \dot{g}(r,t) \) cancel out. This leaves us with the simplified expression:
\[
\nabla^2 F = - 4 \pi \delta(x) \int_{\frac{r}{c} - \epsilon_1}^{\frac{r}{c} + \epsilon_2} \delta(t) \, dt
\]

\item[xiii] The Dirac delta function integrates to 1 over any interval containing $t=0$. 
\[
\int_{\frac{r}{c} - \epsilon_1}^{\frac{r}{c} + \epsilon_2} \delta(t) \, dt = \int_{- \epsilon_1}^{\epsilon_2} \delta(t) \, dt = 1
\]
This reduces the expression for $\nabla^2 F$ to 
\[
\nabla^2 F = - 4 \pi \delta(x)
\]

\item[xiv] Using the green's function property that $\nabla^2 \left( \frac{1}{r} \right) = - 4 \pi \delta(x)$ we conclude that 
\[
F(r, \epsilon_1, \epsilon_2) = \frac{1}{r} \int_{- \epsilon_1}^{\epsilon_2} \delta(t) \, dt
\]
From (iv), we can show that 
\[
4 \pi c^2 \int_{- \epsilon_1}^{\epsilon_2} f(\tau) \, d\tau = \int_{- \epsilon_1}^{\epsilon_2} \delta(t) \, dt
\]
for all \( (\epsilon_1, \epsilon_2) \). Hence, \( f(\tau) = \frac{\delta(\tau)}{4 \pi c^2} \) and 
\[
g(r, t) = g(x, t) = \frac{1}{4 \pi c^2 |x|} \delta\left(t - \frac{|x|}{c}\right)
\]

\end{enumerate} 

---

\vspace{10em}
  

3. Verify that properties (i)-(iv) of LamÃ©'s theorem as defined in AR Section 4.1.1 are satisfied.
    i. $$u = \nabla \phi + \nabla \times \psi$$
    ii. $$\nabla \cdot \psi = 0$$
    iii. $$ \ddot{\phi} = \frac{\Phi}{\rho} + \alpha^2 \nabla^2 \phi \ \ \ \ \    \left( \text{with } \alpha^2 = \frac{\lambda + 2 \mu}{\rho} \right)$$
    iv. $$ \ddot{\psi} = \frac{\Psi}{\rho} + \beta^2 \nabla^2 \psi \ \ \ \ \    \left( \text{with } \beta^2 = \frac{\mu}{\rho} \right)$$